
"""
# Explanation

## Standard Basis

The standard orthonormal right-handed basis vectors are:

- ğ¢ = [1, 0, 0]  
- ğ£ = [0, 1, 0]  
- ğ¤ = [0, 0, 1]

## Tangent Basis

At each point on a surface, we define a tangential plane.
The tangent basis vectors are defined in terms of the standard basis:

- ğâ‚ = aâ‹…ğ¢ + bâ‹…ğ£ + câ‹…ğ¤  
- ğâ‚‚ = dâ‹…ğ¢ + eâ‹…ğ£ + fâ‹…ğ¤  
- ğâ‚ƒ = gâ‹…ğ¢ + hâ‹…ğ£ + iâ‹…ğ¤

These vectors form a right-handed orthonormal basis where:

â€–ğâ‚â€– = â€–ğâ‚‚â€– = â€–ğâ‚ƒâ€– = â€–ğ¢â€– = â€–ğ£â€– = â€–ğ¤â€– = 1

Both bases share the same origin.

## Vector Representation

Let ğ© âˆˆ â„Â³ be a geometric vector with two coordinate representations:

- In the standard basis:  ğ© = [x, y, z] = xâ‹…ğ¢ + yâ‹…ğ£ + zâ‹…ğ¤  
- In the tangent basis:   ğ® = [u, v, w] = uâ‹…ğâ‚ + vâ‹…ğâ‚‚ + wâ‹…ğâ‚ƒ

Here, ğ© and ğ® represent the same vector. The rightmost expressions are equal, 
but the bracketed expressions by themselves leave out which base they are defined in.

## Constraints

- ğâ‚ lies in the xz-plane â‡’ b = 0  
- ğâ‚ points in the positive x direction â‡’ a â‰¥ 0

## Transformation from tangent to standard basis

Let P be the 3Ã—3 matrix whose columns are the tangent basis vectors expressed in the standard basis:
         
    P = [ğâ‚ ğâ‚‚ ğâ‚ƒ] = 
        [a  d  g;
         0  e  h;
         c  f  i]

Then for any vector ğ© âˆˆ â„Â³ with coordinates ğ® = [u, v, w] in the tangent basis, 
the corresponding standard basis coordinates are:

    ğ© = P * ğ® =
        [a   d   g;
         0   e   h;
         c   f   i] * [u;
                      v;
                      w] =
         uğâ‚ + vğâ‚‚ + wğâ‚ƒ


Given ğ® = [u, v, w], the standard basis coordinates ğ© = [x, y, z] are:

    x = aÂ·u + dÂ·v + gÂ·w
    y = eÂ·v + hÂ·w
    z = cÂ·u + fÂ·v + iÂ·w

## Transformation from standard to tangent basis

As defined above, P is a real, square, orthogonal matrix. Therefore, its inverse equals its transpose:

    Pâ»Â¹ = Páµ€ = 
           [a   0   c;
            d   e   f;
            g   h   i]

This simplifies conversion from standard basis coordinates ğ© to tangent basis coordinates ğ®:

    ğ® = Pâ»Â¹ * ğ© = Páµ€ * ğ©

Each component of ğ® represents how much of ğâ‚, ğâ‚‚ or ğâ‚ƒ is present in ğ©. In other words, ğ® gives the unique coefficients such that:

    ğ© = uÂ·ğâ‚ + vÂ·ğâ‚‚ + wÂ·ğâ‚ƒ

Given ğ© = [x, y, z], the tangent basis coordinates ğ® = [u, v, w] are:

    u = aÂ·x +     cÂ·z
    v = dÂ·x + eÂ·y + fÂ·z
    w = gÂ·x + hÂ·y + iÂ·z

"""
foo



"""
# Reversible projection of an angle to the tangent plane

Let ğ© be a vector on the unit circle in the xy-plane, centered at the origin, rotating around the z-axis (ğ¤). 
It represents an angle Î± measured from ğ¢ counterclockwise:

    ğ© = [cos(Î±), sin(Î±), 0] = cos(Î±)â‹…ğ¢ + sin(Î±)â‹…ğ£ 

Let ğª be a vertical vector (parallel with ğ¤), chosen such that the sum ğ« = ğ© + ğª lies in the tangent 
plane (ğâ‚, ğâ‚‚):

    ğª = [0, 0, z], âˆ£ ğ« = ğ© + ğª âˆˆ span(ğâ‚, ğâ‚‚)

Expanding:

    ğ« = cos(Î±)Â·ğ¢ + sin(Î±)Â·ğ£ + zÂ·ğ¤


Substituting ğ¢, ğ£, and ğ¤ with ğâ‚, ğâ‚‚, and ğâ‚ƒ:

    ğ« = cos(Î±)(aÂ·ğâ‚ + dÂ·ğâ‚‚ + gÂ·ğâ‚ƒ)
        + sin(Î±)(eÂ·ğâ‚‚ + hÂ·ğâ‚ƒ)
        + zÂ·(gÂ·ğâ‚ + hÂ·ğâ‚‚ + iÂ·ğâ‚ƒ)

Collecting terms:

    ğ« = (aÂ·cos(Î±) + zÂ·g)â‹…ğâ‚  +  
        (dÂ·cos(Î±) + eÂ·sin(Î±) + zÂ·h)â‹…ğâ‚‚  +
        (gÂ·cos(Î±) + hÂ·sin(Î±) + zÂ·i)â‹…ğâ‚ƒ

Because ğ« lies in the uv plane, we solve for z, requiring the ğâ‚ƒ component to vanish:

    (gÂ·cos(Î±) + hÂ·sin(Î±) + zÂ·i) = 0
    â‡’ z = -(gÂ·cos(Î±) + hÂ·sin(Î±)) / i
    where  i â‰  0.

Recall that ğâ‚ƒ = gÂ·ğ¢ + hÂ·ğ£ + iÂ·ğ¤ â€” that is, i is the z-component of the tangent plane normal 
in standard coordinates. If i = 0, then ğâ‚ƒ lies entirely in the xy-plane, and the tangent plane 
is vertical. In this case, projecting along the z-axis onto the tangent plane is 
undefined. This is consistent with expectations: for a surface defined as a heightfield 
(a "2.5D" surface), the tangent plane is never vertical, so i â‰  0 is a reasonable and 
typical assumption.

Note: Small values of i (close to zero) may amplify numerical errors in floating-point implementations, affecting the accuracy of z and Ï†.

With this z, the ğâ‚ƒ component of ğ« vanishes, so ğ« lies in the tangent plane.

    z = -(gÂ·cos(Î±) + hÂ·sin(Î±)) / i
    âˆ§
    ğ« = (aÂ·cos(Î±) + zÂ·g)â‹…ğâ‚ + (dÂ·cos(Î±) + eÂ·sin(Î±) + zÂ·h)â‹…ğâ‚‚ 

Then we define Ï• to be the angle from ğâ‚ to the direction of ğ« within the tangent plane. It is computed by:
    
    Ï• = atan(dÂ·cos(Î±) + eÂ·sin(Î±) + zÂ·h, aÂ·cos(Î±) + zÂ·g)

This represents the projected angle of Î± into the tangent plane along the z-axis. 
This is a coordinate-driven construction, not a universal projection of angle
between planes. It differs from decomposing rotational vectors such as torque and spin.

# Projection of an angle from the tangent plane to the xy plane

This describes the inverse of the earlier projection. Here, we project angle Ï•
along the same axis, z || ğ¤, with Î± as output. The operation is reversible for 
i â‰  0, but numerical precision may affect results when i is small.

Let ğ® be a vector on the unit circle in the tangent plane, centered at the origin. 
It represents an angle Ï• measured from ğâ‚ counterclockwise:

    ğ® = [u, v, w] = [cos(Ï•), sin(Ï•), 0]

We already [deduced](##_transformation_from_tangent_to_standard_basis) how to express 
the same vector in the standard basis:
    ğ© = [aÂ·u + dÂ·v + gÂ·w, eÂ·v + hÂ·w, cÂ·u + fÂ·v + iÂ·w]

Substituting components of ğ®:

    ğ© = [aÂ·cos(Ï•) + dÂ·sin(Ï•), 
         eÂ·sin(Ï•), 
         cÂ·cos(Ï•) + fÂ·sin(Ï•)]

We now project ğ© along the z axis onto the xy-plane, which amounts to ignoring the third component.
The projected point lies on a ray from origin, and we define Î± as the angle this ray makes 
with the x-axis:

    Î± = atan(eÂ·sin(Ï•), aÂ·cos(Ï•) + dÂ·sin(Ï•))

"""
faa